# Important results

## Matrices

**Prove:**$\bold{(A^{-1})'}=\bold{(A')^{-1}}$

---
**Prove:**$\bold{(AB)'}=\bold{(B'A')}$

---

**Prove:** $\mathbb{E}[\text{Tr}(\bold{X})]=\text{Tr}(\mathbb{E}[\bold{X}])$.
$$
\begin{align*}
    \text{Tr}(\bold{X})&=\sum_{i=1}^nx_{ii},\\
    \mathbb{E}[\text{Tr}(\bold{X})]&=\mathbb{E}[\sum_{i=1}^nx_{ii}],\\
    \mathbb{E}[\text{Tr}(\bold{X})]&=\sum_{i=1}^n\mathbb{E}[x_{ii}].\\
\end{align*}
$$
$\sum_{i=1}^n\mathbb{E}[x_{ii}]$ is equivalent to $\text{Tr}(\mathbb{E}[\bold{X}])$, therefore
$$
\begin{align*}
    \mathbb{E}[\text{Tr}(\bold{X})]&=\sum_{i=1}^n\mathbb{E}[x_{ii}]=\text{Tr}(\mathbb{E}[\bold{X}]).\hspace{15px}\blacksquare\\
\end{align*}
$$